theories/ItoW.v
@@ -1,13 +1,12 @@
 
 From Coq Require Import Bool String List BinPos Compare_dec Omega.
-From Template
-Require Import Ast utils monad_utils Typing Checker.
 From Translation
      Require Import util Sorts SAst SLiftSubst WAst WLiftSubst
      SCommon ITyping ITypingLemmata
      WTyping WChecker WLemmata Quotes.
 From TypingFlags Require Import Loader.
-Import MonadNotation ListNotations.
+Import ListNotations.
+Open Scope string_scope.
 
 Section Translation.
 
@@ -57,13 +56,15 @@ Fixpoint tsl (t : sterm) : wterm :=
   | _ => wAx "todo"
   end.
 
-Fixpoint tsl_glob (Σ : sglobal_context) : wglobal_context :=
+Program Fixpoint tsl_glob (Σ : sglobal_context) : wglobal_context :=
   match Σ with
   | d :: Σ =>
-    {| dname := d.(SCommon.dname) ; dtype := tsl d.(SCommon.dtype) ; dbody := ?? |}
+    {| dname := d.(SCommon.dname) ; dtype := tsl d.(SCommon.dtype) ; dbody := _ |}
     :: tsl_glob Σ
   | nil => nil
   end.
+Next Obligation.
+Admitted.
 
 Fixpoint tsl_ctx (Γ : scontext) : wcontext :=
   match Γ with
@@ -111,195 +112,195 @@ Proof.
   apply tsl_lift.
 Defined.
 
-Lemma tsl_lookup :
-  forall {Σ id ty},
-    SCommon.lookup_glob Σ id = Some ty ->
-    lookup_glob (tsl_glob Σ) id = Some (tsl ty).
-Proof.
-  intro Σ. induction Σ ; intros id ty eq.
-  - cbn in eq. discriminate eq.
-  - revert eq. cbn. case_eq (ident_eq id (SCommon.dname a)).
-    + intros e eq. inversion eq. subst. reflexivity.
-    + intros e eq. eapply IHΣ. assumption.
-Defined.
+(* Lemma tsl_lookup : *)
+(*   forall {Σ id ty}, *)
+(*     SCommon.lookup_glob Σ id = Some ty -> *)
+(*     lookup_glob (tsl_glob Σ) id = Some (tsl ty). *)
+(* Proof. *)
+(*   intro Σ. induction Σ ; intros id ty eq. *)
+(*   - cbn in eq. discriminate eq. *)
+(*   - revert eq. cbn. case_eq (ident_eq id (SCommon.dname a)). *)
+(*     + intros e eq. inversion eq. subst. reflexivity. *)
+(*     + intros e eq. eapply IHΣ. assumption. *)
+(* Defined. *)
 
-Lemma nl_tsl :
-  forall {u v},
-    Equality.nl u = Equality.nl v ->
-    WEquality.nl (tsl u) = WEquality.nl (tsl v).
-Proof.
-  intro u. induction u ; intros v eq.
-  all: destruct v ; simpl in eq ; try discriminate eq.
-  all: try (
-    cbn ; inversion eq ; f_equal ;
-    try eapply IHu ;
-    try eapply IHu1 ; try eapply IHu2 ;
-    try eapply IHu3 ; try eapply IHu4 ;
-    try eapply IHu5 ; try eapply IHu6 ;
-    assumption
-  ).
-Defined.
+(* Lemma nl_tsl : *)
+(*   forall {u v}, *)
+(*     Equality.nl u = Equality.nl v -> *)
+(*     WEquality.nl (tsl u) = WEquality.nl (tsl v). *)
+(* Proof. *)
+(*   intro u. induction u ; intros v eq. *)
+(*   all: destruct v ; simpl in eq ; try discriminate eq. *)
+(*   all: try ( *)
+(*     cbn ; inversion eq ; f_equal ; *)
+(*     try eapply IHu ; *)
+(*     try eapply IHu1 ; try eapply IHu2 ; *)
+(*     try eapply IHu3 ; try eapply IHu4 ; *)
+(*     try eapply IHu5 ; try eapply IHu6 ; *)
+(*     assumption *)
+(*   ). *)
+(* Defined. *)
 
-Open Scope i_scope.
+(* Open Scope i_scope. *)
 
-Ltac lift_sort :=
-  match goal with
-  | |- _ ;;; _ |-w lift ?n ?k ?t : ?S => change S with (lift n k S)
-  | |- _ ;;; _ |-w ?t { ?n := ?u } : ?S => change S with (S {n := u})
-  end.
+(* Ltac lift_sort := *)
+(*   match goal with *)
+(*   | |- _ ;;; _ |-w lift ?n ?k ?t : ?S => change S with (lift n k S) *)
+(*   | |- _ ;;; _ |-w ?t { ?n := ?u } : ?S => change S with (S {n := u}) *)
+(*   end. *)
 
-Ltac callih :=
-  match goal with
-  | h : let _ := _ in
-        let _ := tsl ?t in
-        let _ := _ in _ -> _ ;;; _ |-w _ : _
-    |- _ ;;; _ |-w tsl ?t : _ =>
-    eapply h
-  end.
+(* Ltac callih := *)
+(*   match goal with *)
+(*   | h : let _ := _ in *)
+(*         let _ := tsl ?t in *)
+(*         let _ := _ in _ -> _ ;;; _ |-w _ : _ *)
+(*     |- _ ;;; _ |-w tsl ?t : _ => *)
+(*     eapply h *)
+(*   end. *)
 
-Ltac wfctx :=
-  first [
-    eassumption
-    | cbn ; eapply wf_snoc ; try assumption
-  ].
+(* Ltac wfctx := *)
+(*   first [ *)
+(*     eassumption *)
+(*     | cbn ; eapply wf_snoc ; try assumption *)
+(*   ]. *)
 
-Ltac ih :=
-  repeat (callih ; wfctx).
+(* Ltac ih := *)
+(*   repeat (callih ; wfctx). *)
 
-Ltac go t' A' :=
-  unfold t', A' ; cbn ;
-  repeat (rewrite ?tsl_lift, ?tsl_subst) ;
-  econstructor ; try assumption ; ih.
+(* Ltac go t' A' := *)
+(*   unfold t', A' ; cbn ; *)
+(*   repeat (rewrite ?tsl_lift, ?tsl_subst) ; *)
+(*   econstructor ; try assumption ; ih. *)
 
-Lemma tsl_sound :
-  forall {Σ Γ t A},
-    let Σ' := tsl_glob Σ in
-    let Γ' := tsl_ctx Γ in
-    let t' := tsl t in
-    let A' := tsl A in
-    type_glob Σ' ->
-    wf Σ' Γ' ->
-    Σ ;;; Γ |-i t : A ->
-    Σ' ;;; Γ' |-w t' : A'.
-Proof.
-  intros Σ Γ t A Σ' Γ' t' A' hg hw h. induction h.
-  all: try solve [go t' A'].
-  - unfold t', A'. cbn. rewrite tsl_lift. unshelve erewrite tsl_safe_nth.
-    + cbn. rewrite tsl_ctx_length. assumption.
-    + econstructor. assumption.
-  - unfold t', A'. cbn. econstructor ; try assumption ; try ih.
-    rewrite <- tsl_subst. ih.
-  - unfold t', A'. repeat (rewrite ?tsl_lift, ?tsl_subst).
-    cbn. econstructor ; try assumption ; try ih.
-    + eapply rename_typed ; try assumption.
-      * eapply IHh4. cbn. repeat eapply wf_snoc ; try assumption.
-        -- ih.
-        -- econstructor.
-           ++ rewrite tsl_lift. lift_sort.
-              eapply typing_lift01 ; try assumption ; ih.
-           ++ rewrite 2!tsl_lift.
-              eapply typing_lift01 ; try assumption ; ih.
-           ++ rewrite tsl_lift. refine (type_Rel _ _ _ _ _).
-              ** wfctx ; ih.
-              ** cbn. auto with arith.
-      * cbn. rewrite 2!tsl_lift. reflexivity.
-      * reflexivity.
-      * repeat eapply wf_snoc ; try assumption ; ih.
-        econstructor.
-        -- lift_sort.
-           eapply typing_lift01 ; try assumption ; ih.
-        -- eapply typing_lift01 ; try assumption ; ih.
-        -- refine (type_Rel _ _ _ _ _).
-           ++ wfctx ; ih.
-           ++ cbn. auto with arith.
-    + repeat (rewrite ?tsl_lift, ?tsl_subst in IHh6). ih.
-  - give_up.
-  - give_up.
-  - give_up.
-  - give_up.
-  - give_up.
-  - give_up.
-  - give_up.
-  - give_up.
-  - give_up.
-  - give_up.
-  - give_up.
-  - give_up.
-  - give_up.
-  - give_up.
-  - give_up.
-  - give_up.
-  - give_up.
-  - give_up.
-  - give_up.
-  - give_up.
-  - give_up.
-  - unfold t', A'. econstructor.
-    + assumption.
-    + eapply tsl_lookup. assumption.
-  - eapply type_rename.
-    + eapply IHh. assumption.
-    + unfold A'. eapply nl_tsl. assumption.
-Admitted.
+(* Lemma tsl_sound : *)
+(*   forall {Σ Γ t A}, *)
+(*     let Σ' := tsl_glob Σ in *)
+(*     let Γ' := tsl_ctx Γ in *)
+(*     let t' := tsl t in *)
+(*     let A' := tsl A in *)
+(*     type_glob Σ' -> *)
+(*     wf Σ' Γ' -> *)
+(*     Σ ;;; Γ |-i t : A -> *)
+(*     Σ' ;;; Γ' |-w t' : A'. *)
+(* Proof. *)
+(*   intros Σ Γ t A Σ' Γ' t' A' hg hw h. induction h. *)
+(*   all: try solve [go t' A']. *)
+(*   - unfold t', A'. cbn. rewrite tsl_lift. unshelve erewrite tsl_safe_nth. *)
+(*     + cbn. rewrite tsl_ctx_length. assumption. *)
+(*     + econstructor. assumption. *)
+(*   - unfold t', A'. cbn. econstructor ; try assumption ; try ih. *)
+(*     rewrite <- tsl_subst. ih. *)
+(*   - unfold t', A'. repeat (rewrite ?tsl_lift, ?tsl_subst). *)
+(*     cbn. econstructor ; try assumption ; try ih. *)
+(*     + eapply rename_typed ; try assumption. *)
+(*       * eapply IHh4. cbn. repeat eapply wf_snoc ; try assumption. *)
+(*         -- ih. *)
+(*         -- econstructor. *)
+(*            ++ rewrite tsl_lift. lift_sort. *)
+(*               eapply typing_lift01 ; try assumption ; ih. *)
+(*            ++ rewrite 2!tsl_lift. *)
+(*               eapply typing_lift01 ; try assumption ; ih. *)
+(*            ++ rewrite tsl_lift. refine (type_Rel _ _ _ _ _). *)
+(*               ** wfctx ; ih. *)
+(*               ** cbn. auto with arith. *)
+(*       * cbn. rewrite 2!tsl_lift. reflexivity. *)
+(*       * reflexivity. *)
+(*       * repeat eapply wf_snoc ; try assumption ; ih. *)
+(*         econstructor. *)
+(*         -- lift_sort. *)
+(*            eapply typing_lift01 ; try assumption ; ih. *)
+(*         -- eapply typing_lift01 ; try assumption ; ih. *)
+(*         -- refine (type_Rel _ _ _ _ _). *)
+(*            ++ wfctx ; ih. *)
+(*            ++ cbn. auto with arith. *)
+(*     + repeat (rewrite ?tsl_lift, ?tsl_subst in IHh6). ih. *)
+(*   - give_up. *)
+(*   - give_up. *)
+(*   - give_up. *)
+(*   - give_up. *)
+(*   - give_up. *)
+(*   - give_up. *)
+(*   - give_up. *)
+(*   - give_up. *)
+(*   - give_up. *)
+(*   - give_up. *)
+(*   - give_up. *)
+(*   - give_up. *)
+(*   - give_up. *)
+(*   - give_up. *)
+(*   - give_up. *)
+(*   - give_up. *)
+(*   - give_up. *)
+(*   - give_up. *)
+(*   - give_up. *)
+(*   - give_up. *)
+(*   - give_up. *)
+(*   - unfold t', A'. econstructor. *)
+(*     + assumption. *)
+(*     + eapply tsl_lookup. assumption. *)
+(*   - eapply type_rename. *)
+(*     + eapply IHh. assumption. *)
+(*     + unfold A'. eapply nl_tsl. assumption. *)
+(* Admitted. *)
 
-Lemma tsl_fresh_glob :
-  forall {id Σ},
-    ITyping.fresh_glob id Σ ->
-    fresh_glob id (tsl_glob Σ).
-Proof.
-  intros id Σ h. induction h.
-  - cbn. constructor.
-  - cbn. econstructor ; assumption.
-Defined.
+(* Lemma tsl_fresh_glob : *)
+(*   forall {id Σ}, *)
+(*     ITyping.fresh_glob id Σ -> *)
+(*     fresh_glob id (tsl_glob Σ). *)
+(* Proof. *)
+(*   intros id Σ h. induction h. *)
+(*   - cbn. constructor. *)
+(*   - cbn. econstructor ; assumption. *)
+(* Defined. *)
 
-Lemma tsl_glob_sound :
-  forall {Σ},
-    ITyping.type_glob Σ ->
-    type_glob (tsl_glob Σ).
-Proof.
-  intros Σ h. induction h.
-  - cbn. econstructor.
-  - cbn. econstructor ; try assumption.
-    + cbn. eapply tsl_fresh_glob. assumption.
-    + cbn. destruct i as [s hh].
-      exists s. change (wSort s) with (tsl (sSort s)).
-      change [] with (tsl_ctx []).
-      eapply tsl_sound ; try assumption.
-      cbn. constructor.
-Defined.
+(* Lemma tsl_glob_sound : *)
+(*   forall {Σ}, *)
+(*     ITyping.type_glob Σ -> *)
+(*     type_glob (tsl_glob Σ). *)
+(* Proof. *)
+(*   intros Σ h. induction h. *)
+(*   - cbn. econstructor. *)
+(*   - cbn. econstructor ; try assumption. *)
+(*     + cbn. eapply tsl_fresh_glob. assumption. *)
+(*     + cbn. destruct i as [s hh]. *)
+(*       exists s. change (wSort s) with (tsl (sSort s)). *)
+(*       change [] with (tsl_ctx []). *)
+(*       eapply tsl_sound ; try assumption. *)
+(*       cbn. constructor. *)
+(* Defined. *)
 
-Lemma tsl_ctx_sound :
-  forall {Σ Γ},
-    ITyping.type_glob Σ ->
-    ITyping.wf Σ Γ ->
-    wf (tsl_glob Σ) (tsl_ctx Γ).
-Proof.
-  intros Σ Γ hg hw. induction hw.
-  - cbn. constructor.
-  - cbn. econstructor ; try eassumption.
-    match goal with
-    | |- _ ;;; _ |-w _ : wSort ?s =>
-      change (wSort s) with (tsl (sSort s))
-    end.
-    eapply tsl_sound ; try eassumption.
-    eapply tsl_glob_sound. assumption.
-Defined.
+(* Lemma tsl_ctx_sound : *)
+(*   forall {Σ Γ}, *)
+(*     ITyping.type_glob Σ -> *)
+(*     ITyping.wf Σ Γ -> *)
+(*     wf (tsl_glob Σ) (tsl_ctx Γ). *)
+(* Proof. *)
+(*   intros Σ Γ hg hw. induction hw. *)
+(*   - cbn. constructor. *)
+(*   - cbn. econstructor ; try eassumption. *)
+(*     match goal with *)
+(*     | |- _ ;;; _ |-w _ : wSort ?s => *)
+(*       change (wSort s) with (tsl (sSort s)) *)
+(*     end. *)
+(*     eapply tsl_sound ; try eassumption. *)
+(*     eapply tsl_glob_sound. assumption. *)
+(* Defined. *)
 
-Corollary tsl_soundness :
-forall {Σ Γ t A},
-    let Σ' := tsl_glob Σ in
-    let Γ' := tsl_ctx Γ in
-    let t' := tsl t in
-    let A' := tsl A in
-    ITyping.type_glob Σ ->
-    Σ ;;; Γ |-i t : A ->
-    Σ' ;;; Γ' |-w t' : A'.
-Proof.
-  intros Σ Γ t A Σ' Γ' t' A' hg h.
-  eapply tsl_sound ; try assumption.
-  - eapply tsl_glob_sound. assumption.
-  - eapply tsl_ctx_sound ; try assumption.
-    eapply ITypingLemmata.typing_wf. eassumption.
-Defined.
+(* Corollary tsl_soundness : *)
+(* forall {Σ Γ t A}, *)
+(*     let Σ' := tsl_glob Σ in *)
+(*     let Γ' := tsl_ctx Γ in *)
+(*     let t' := tsl t in *)
+(*     let A' := tsl A in *)
+(*     ITyping.type_glob Σ -> *)
+(*     Σ ;;; Γ |-i t : A -> *)
+(*     Σ' ;;; Γ' |-w t' : A'. *)
+(* Proof. *)
+(*   intros Σ Γ t A Σ' Γ' t' A' hg h. *)
+(*   eapply tsl_sound ; try assumption. *)
+(*   - eapply tsl_glob_sound. assumption. *)
+(*   - eapply tsl_ctx_sound ; try assumption. *)
+(*     eapply ITypingLemmata.typing_wf. eassumption. *)
+(* Defined. *)
 
 End Translation.
