theories/XChecking.v
@@ -2,7 +2,6 @@
 
 From Coq Require Import Bool String List BinPos Compare_dec Omega.
 From Equations Require Import Equations DepElimDec.
-From Template Require Import utils Ast Typing Checker.
 From Translation Require Import util Quotes Sorts SAst SLiftSubst SCommon
      ITyping ITypingInversions ITypingLemmata ITypingAdmissible XTyping
      FundamentalLemma Translation FinalTranslation FullQuote
