theories/monad_utils.v
@@ -1,0 +1,108 @@
+Require Import List.
+
+Set Universe Polymorphism.
+
+Class Monad@{d c} (m : Type@{d} -> Type@{c}) : Type :=
+{ ret : forall {t : Type@{d}}, t -> m t
+; bind : forall {t u : Type@{d}}, m t -> (t -> m u) -> m u
+}.
+
+Class MonadExc E (m : Type -> Type) : Type :=
+{ raise : forall {T}, E -> m T
+; catch : forall {T}, m T -> (E -> m T) -> m T
+}.
+
+
+Delimit Scope monad_scope with monad.
+ 
+Notation "c >>= f" := (@bind _ _ _ _ c f) (at level 50, left associativity) : monad_scope.
+Notation "f =<< c" := (@bind _ _ _ _ c f) (at level 51, right associativity) : monad_scope.
+ 
+Notation "x <- c1 ;; c2" := (@bind _ _ _ _ c1 (fun x => c2))
+  (at level 100, c1 at next level, right associativity) : monad_scope.
+ 
+Notation "e1 ;; e2" := (_ <- e1%monad ;; e2%monad)%monad
+  (at level 100, right associativity) : monad_scope.
+
+
+Instance option_monad : Monad option :=
+  {| ret A a := Some a ;
+     bind A B m f :=
+       match m with
+       | Some a => f a
+       | None => None
+       end
+  |}.
+
+Open Scope monad.
+
+Section MapOpt.
+  Context {A} (f : A -> option A).
+
+  Fixpoint mapopt (l : list A) : option (list A) :=
+    match l with
+    | nil => ret nil
+    | x :: xs => x' <- f x ;;
+                xs' <- mapopt xs ;;
+                ret (x' :: xs')
+    end.
+End MapOpt.
+
+Section MonadOperations.
+  Context {T} {M : Monad T}.
+  Context {A B} (f : A -> T B).
+  Fixpoint monad_map (l : list A)
+    : T (list B)
+    := match l with
+       | nil => ret nil
+       | x :: l => x' <- f x ;;
+                  l' <- monad_map l ;;
+                  ret (x' :: l')
+       end.
+
+  Context (g : A -> B -> T A).
+  Fixpoint monad_fold_left (l : list B) (x : A) : T A
+    := match l with
+       | nil => ret x
+       | y :: l => x' <- g x y ;;
+                   monad_fold_left l x'
+       end.
+
+  Context (h : nat -> A -> T B).
+  Fixpoint monad_map_i_aux (n0 : nat) (l : list A) : T (list B)
+    := match l with
+       | nil => ret nil
+       | x :: l => x' <- (h n0 x) ;;
+                   l' <- (monad_map_i_aux (S n0) l) ;;
+                   ret (x' :: l')
+       end.
+
+  Definition monad_map_i := @monad_map_i_aux 0.
+End MonadOperations.
+
+
+(* Error monad *)
+Inductive result E A :=
+| Success : A -> result E A
+| Error : E -> result E A.
+
+Arguments Success {_ _} _.
+Arguments Error {_ _} _.
+
+Instance error_monad E : Monad (result E) :=
+  {| ret A a := Success a ;
+     bind A B m f :=
+       match m with
+       | Success a => f a
+       | Error e => Error e
+       end
+  |}.
+
+Instance monad_exc E : MonadExc E (result E) :=
+  { raise A e := Error e;
+    catch A m f :=
+      match m with
+      | Success a => m
+      | Error t => f t
+      end
+  }.
